src/tls/Model.AE.fst
@@ -1,0 +1,156 @@
+module Model.AE
+include Model.AEAD
+
+module HST = FStar.HyperStack.ST
+module B = LowStar.Buffer
+module CL = C.Loops
+module MU = Model.Utils
+module SC = Spec.AEAD
+module F = Flags
+module E = EverCrypt
+module ES = EverCrypt.Specs
+module U32 = FStar.UInt32
+
+inline_for_extraction
+let iv_len = 12ul
+
+inline_for_extraction
+noextract
+let random_sample
+  (len: U32.t)
+  (out: B.buffer SC.uint8 { B.len out == len })
+: HST.Stack unit
+  (requires (fun h -> B.live h out))
+  (ensures (fun h _ h' -> B.modifies (B.loc_buffer out) h h'))
+= let h = HST.get () in
+  assume (ES.random_sample_pre h);
+  E.random_sample len out
+
+inline_for_extraction
+noextract
+let iv_length = 12
+
+let rec regenerate_iv
+  (#a: SC.supported_alg)
+  (#phi: plain_pred)
+  (s: state a phi) // key
+  (out: B.buffer SC.uint8)
+: HST.Stack (s: SC.iv a { Seq.length s == iv_length })
+  (requires (fun h ->
+    B.loc_disjoint (B.loc_buffer out) (footprint s) /\
+    B.live h out /\
+    B.len out == iv_len /\
+    invariant h s /\
+    F.model == true
+  ))
+  (ensures (fun h res h' ->
+    B.modifies (B.loc_buffer out) h h' /\
+    res == B.as_seq h' out /\
+    (F.ideal_iv == true ==> fresh_iv h' s res)
+  ))
+= let h0 = HST.get () in
+  random_sample iv_len out;
+  let iv = MU.get_buffer out iv_len in
+  let h1 = HST.get () in
+  frame_invariant h0 s (B.loc_buffer out) h1;
+  if F.ideal_iv
+  then begin
+    let cond = is_fresh_iv s iv in
+    let h' = HST.get () in
+    frame_fresh_iv h1 s iv B.loc_none h' ;
+    if cond
+    then iv
+    else begin
+      frame_invariant h1 s B.loc_none h' ;
+      regenerate_iv s out
+    end
+  end else iv
+
+let generate_iv
+  (#a: SC.supported_alg)
+  (#phi: plain_pred)
+  (s: state a phi) // key
+: HST.Stack (s: SC.iv a { Seq.length s == iv_length })
+  (requires (fun h ->
+    F.model == true /\
+    invariant h s
+  ))
+  (ensures (fun h iv h' ->
+    B.modifies B.loc_none h h' /\
+    (F.ideal_iv == true ==> fresh_iv h s iv)
+  ))
+= let h = HST.get () in
+  invariant_loc_in_footprint h s;
+  HST.push_frame ();
+  let b = B.alloca (Lib.IntTypes.mk_int 0 <: SC.uint8) iv_len in
+  let h1 = HST.get () in
+  frame_invariant h s B.loc_none h1 ;
+  let res = regenerate_iv s b in
+  let h2 = HST.get () in
+  frame_fresh_iv h s res B.loc_none h2;
+  HST.pop_frame ();
+  res
+
+val encrypt
+  (#a: SC.supported_alg)
+  (#phi: plain_pred)
+  (s: state a phi) // key
+  (plain: SC.plain a)
+: HST.Stack (s: Seq.seq SC.uint8 { Seq.length s == iv_length + Seq.length plain + SC.tag_length a }) 
+  (requires (fun h ->
+    Flags.model == true /\
+    invariant h s /\
+    phi plain
+  ))
+  (ensures (fun h cipher h' -> 
+    B.modifies (footprint s) h h' /\
+    Seq.length cipher <= iv_length + SC.max_length a + SC.tag_length a /\ (
+    let iv = Seq.slice cipher 0 iv_length in
+    invariant h' s /\
+    (Flags.ideal_AEAD == false ==>
+      SC.encrypt (state_kv s) iv Seq.empty plain == Seq.slice cipher iv_length (Seq.length cipher)
+  ))))
+
+let encrypt
+  #a #phi s plain
+= let h = HST.get () in
+  let iv = generate_iv s in
+  let h1 = HST.get () in
+  frame_invariant h s B.loc_none h1;
+  frame_fresh_iv h s iv B.loc_none h1;
+  let cipher = encrypt s iv plain in
+  let res = Seq.append iv cipher in
+  assert (Seq.slice res 0 iv_length `Seq.equal` iv);
+  assert (Seq.slice res iv_length (Seq.length res) `Seq.equal` cipher);
+  res
+
+val decrypt
+  (#a: SC.supported_alg)
+  (#phi: plain_pred)
+  (s: state a phi) // key
+  (cipher: SC.cipher a { Seq.length cipher >= iv_length + SC.tag_length a /\ Seq.length cipher <= iv_length + SC.max_length a + SC.tag_length a })
+: HST.Stack (option (plain: Seq.seq SC.uint8 { Seq.length cipher == iv_length + Seq.length plain + SC.tag_length a }))
+  (requires (fun h ->
+    Flags.model == true /\
+    invariant h s
+  ))
+  (ensures (fun h res h' ->
+    B.modifies (footprint s) h h' /\ (
+    let cipher' = Seq.slice cipher iv_length (Seq.length cipher) in
+    let iv = Seq.slice cipher 0 iv_length in
+    (Flags.ideal_AEAD == false ==> (
+      SC.decrypt (state_kv s) iv Seq.empty cipher' == res
+    )) /\
+    invariant h' s /\
+    begin match res with
+    | None -> True
+    | Some plain ->
+      (Flags.ideal_AEAD == true ==> phi plain)
+    end
+  )))
+
+let decrypt
+  #a #phi s cipher
+= let iv' = Seq.slice cipher 0 iv_length in
+  let cipher' = Seq.slice cipher iv_length (Seq.length cipher) in
+  decrypt s iv' cipher'
